working mono ITE for bd

f.ml
@@ -1,140 +1,22 @@
 structure test : sig
-  type char
-  type 'a set
-  type ('a, 'b) sum
-  type 'a bd
-  val fail : 'a bd
-  val parse : 'a bd -> char list -> ('a * char list) option
-  val t : (char * char list) option
+  type 'a enum
+  val t : 'c enum -> ('a -> 'b -> bool) -> ('c -> 'a) -> ('c -> 'b) -> bool
 end = struct
 
-fun equal_bool p true = p
-  | equal_bool p false = not p
-  | equal_bool true p = p
-  | equal_bool false p = not p;
+type 'a finite = {};
 
-datatype char = Chara of bool * bool * bool * bool * bool * bool * bool * bool;
+type 'a enum =
+  {finite_enum : 'a finite, enum : 'a list, enum_all : ('a -> bool) -> bool,
+    enum_ex : ('a -> bool) -> bool};
+val finite_enum = #finite_enum : 'a enum -> 'a finite;
+val enum = #enum : 'a enum -> 'a list;
+val enum_all = #enum_all : 'a enum -> ('a -> bool) -> bool;
+val enum_ex = #enum_ex : 'a enum -> ('a -> bool) -> bool;
 
-fun equal_chara (Chara (x1, x2, x3, x4, x5, x6, x7, x8))
-  (Chara (y1, y2, y3, y4, y5, y6, y7, y8)) =
-  equal_bool x1 y1 andalso
-    (equal_bool x2 y2 andalso
-      (equal_bool x3 y3 andalso
-        (equal_bool x4 y4 andalso
-          (equal_bool x5 y5 andalso
-            (equal_bool x6 y6 andalso
-              (equal_bool x7 y7 andalso equal_bool x8 y8))))));
+fun all A_ p = enum_all A_ p;
 
-type 'a equal = {equal : 'a -> 'a -> bool};
-val equal = #equal : 'a equal -> 'a -> 'a -> bool;
+fun fun_ord C_ ord f g = all C_ (fn x => ord (f x) (g x));
 
-val equal_char = {equal = equal_chara} : char equal;
-
-datatype 'a set = Set of 'a list | Coset of 'a list;
-
-datatype ('a, 'b) sum = Inl of 'a | Inr of 'b;
-
-datatype 'a bd =
-  Abs_bd of
-    (((char list), 'a) sum -> (('a * char list), (char list)) sum option);
-
-fun id x = (fn xa => xa) x;
-
-fun eq A_ a b = equal A_ a b;
-
-val bot_set : 'a set = Set [];
-
-fun one_char_printer c = SOME [c];
-
-fun one_char_parser [] = NONE
-  | one_char_parser (c :: cs) = SOME (c, cs);
-
-fun map_option f NONE = NONE
-  | map_option f (SOME x2) = SOME (f x2);
-
-fun bdc_aux parser printer (Inl s) = map_option Inl (parser s)
-  | bdc_aux parser printer (Inr t) = map_option Inr (printer t);
-
-fun bdc xb xc = Abs_bd (bdc_aux xb xc);
-
-val one_char : char bd = bdc one_char_parser one_char_printer;
-
-fun return A_ t =
-  bdc (fn i => SOME (t, i)) (fn ta => (if eq A_ ta t then SOME [] else NONE));
-
-val fail : 'a bd = bdc (fn _ => NONE) (fn _ => NONE);
-
-fun projl (Inl x1) = x1;
-
-fun pr_map f (pr, pl) = (f pr, pl);
-
-fun opr_map f NONE = NONE
-  | opr_map f (SOME p) = SOME (pr_map f p);
-
-fun projr (Inr x2) = x2;
-
-fun print_aux bd_aux s = map_option projr (bd_aux (Inr s));
-
-fun rep_bd (Abs_bd x) = x;
-
-fun print xa = print_aux (rep_bd xa);
-
-fun parse_aux bd_aux s = map_option projl (bd_aux (Inl s));
-
-fun parse xa = parse_aux (rep_bd xa);
-
-fun transform a2b b2a bd = bdc (opr_map a2b o parse bd) (print bd o b2a);
-
-fun binda NONE f = NONE
-  | binda (SOME x) f = f x;
-
-fun ite_printer pa a2pb pc b2a (Inl b) =
-  let
-    val a = b2a b;
-  in
-    binda (pa a) (fn pra => binda (a2pb a b) (fn prb => SOME (pra @ prb)))
-  end
-  | ite_printer pa a2pb pc b2a (Inr c) = pc c;
-
-fun ite_parser a a2b c i =
-  (case a i of NONE => opr_map Inr (c i)
-    | SOME (r, l) => opr_map Inl (a2b r l));
-
-fun ite a a2b c b2a =
-  bdc (ite_parser (parse a) (parse o a2b) (parse c))
-    (ite_printer (print a) (print o a2b) (print c) b2a);
-
-fun bind a a2bd b2a = transform projl Inl (ite a a2bd fail b2a);
-
-fun char_if p =
-  bind one_char (fn r => (if p r then return equal_char r else fail)) id;
-
-fun membera A_ [] y = false
-  | membera A_ (x :: xs) y = eq A_ x y orelse membera A_ xs y;
-
-fun member A_ x (Coset xs) = not (membera A_ xs x)
-  | member A_ x (Set xs) = membera A_ xs x;
-
-fun in_set s = char_if (fn i => member equal_char i s);
-
-fun removeAll A_ x [] = []
-  | removeAll A_ x (y :: xs) =
-    (if eq A_ x y then removeAll A_ x xs else y :: removeAll A_ x xs);
-
-fun inserta A_ x xs = (if membera A_ xs x then xs else x :: xs);
-
-fun insert A_ x (Coset xs) = Coset (removeAll A_ x xs)
-  | insert A_ x (Set xs) = Set (inserta A_ x xs);
-
-val t : (char * char list) option =
-  parse (in_set
-          (insert equal_char
-            (Chara (true, false, false, false, false, true, true, false))
-            bot_set))
-    [Chara (true, false, false, false, false, true, true, false),
-      Chara (false, false, false, false, true, true, true, false),
-      Chara (false, false, false, false, true, true, true, false),
-      Chara (false, false, true, true, false, true, true, false),
-      Chara (true, false, true, false, false, true, true, false)];
+fun t C_ = fun_ord C_;
 
 end; (*struct test*)
